feat(HOL_To_HOL_Nat): Mechanically redefine no-assumption variants of compiled HOL-Nat functions (#14)
* function to remove conditions and TYPE args

* write some functions

* basename support

* cook a bogstandard brew

* clean up

* add a comment, clean up

* remove unnecessary printouts

HOL_To_IMP_Minus/Refinements/HOL_To_IMP_Minus_Datatypes.thy
@@ -2,79 +2,328 @@
 theory HOL_To_IMP_Minus_Datatypes
   imports
     HOL_To_IMP_Minus_Arithmetics
+    "HOL-Data_Structures.Cmp"
 begin
+
+datatype_compile_nat cmp_val
 
 locale HOL_To_HOL_Nat =
   notes transport_eq_id.partial_equivalence_rel_equivalenceI[per_intro del]
   and transport_eq_restrict_id.partial_equivalence_rel_equivalence[per_intro del]
 begin
 
-fun rev_tail_aux :: "'a list \<Rightarrow> 'a list \<Rightarrow> 'a list" where
-"rev_tail_aux [] acc = acc" |
-"rev_tail_aux (x # xs) acc = rev_tail_aux xs (x # acc)"
+section \<open>Pair\<close>
 
-lemma rev_tail_aux_eq_rev_append [simp]: "rev_tail_aux xs acc = rev xs @ acc"
-  by (induction xs arbitrary: acc) auto
+function_compile_nat fst_def
+function_compile_nat snd_def
 
-case_of_simps rev_tail_aux_eq_case : rev_tail_aux.simps
-function_compile_nat rev_tail_aux_eq_case
-print_theorems
-definition "rev_tail xs \<equiv> rev_tail_aux xs []"
 
-lemma rev_tail_eq_rev [simp]: "rev_tail xs = rev xs"
-  unfolding rev_tail_def by simp
+section\<open>Three-way compare\<close>
+
+(* would require ord typeclass *)
+(* function_compile_nat cmp_def *)
+
+
+section\<open>Comparison (nat)\<close>
+
+fun "leq_aux" :: "nat \<Rightarrow> nat \<Rightarrow> bool" where
+  "leq_aux 0 _ = True" |
+  "leq_aux (Suc _) 0 = False" |
+  "leq_aux (Suc x) (Suc y) = leq_aux x y"
+
+lemma leq_eq_leq_aux: "(x \<le> y) \<equiv> leq_aux x y"
+  by (induction x y rule: leq_aux.induct) auto
+
+case_of_simps leq_aux_eq : leq_aux.simps
+function_compile_nat leq_aux_eq
+function_compile_nat leq_eq_leq_aux
+
+
+section \<open>Option\<close>
+
+paragraph \<open>is_some\<close>
+
+fun is_some :: "'a option \<Rightarrow> bool" where
+  "is_some (Some _) = True" |
+  "is_some None = False"
+
+case_of_simps is_some_eq : is_some.simps
+function_compile_nat is_some_eq
+
+
+paragraph \<open>get_some\<close>
+
+fun get_some :: "'a \<Rightarrow> 'a option \<Rightarrow> 'a" where
+  "get_some _ (Some x) = x" |
+  "get_some d _ = d"
+
+case_of_simps get_some_eq : get_some.simps
+function_compile_nat get_some_eq
+
+
+section\<open>List\<close>
+
+paragraph \<open>length\<close>
+
+fun length_aux :: "nat \<Rightarrow> 'a list \<Rightarrow> nat" where
+  "length_aux acc [] = acc" |
+  "length_aux acc (_ # xs) = length_aux (Suc acc) xs"
+
+lemma length_eq_length_aux: "List.length xs + k = length_aux k xs"
+  by (induction k xs rule: length_aux.induct) auto
+
+lemma length_eq_length_aux0: "List.length xs = length_aux 0 xs"
+  by (rule length_eq_length_aux[where k = 0, simplified])
+
+case_of_simps length_aux_eq : length_aux.simps
+function_compile_nat length_aux_eq
+function_compile_nat length_eq_length_aux0
+
+
+paragraph\<open>compare_lengths\<close>
+
+fun compare_lengths :: "'a list \<Rightarrow> 'b list \<Rightarrow> cmp_val" where
+  "compare_lengths [] [] = EQ" |
+  "compare_lengths [] _ = LT" |
+  "compare_lengths _ [] = GT" |
+  "compare_lengths (_ # xs) (_ # ys) = compare_lengths xs ys"
+
+case_of_simps compare_lengths_eq : compare_lengths.simps
+function_compile_nat compare_lengths_eq
+
+
+paragraph \<open>rev_aux\<close>
+
+fun rev_aux :: "'a list \<Rightarrow> 'a list \<Rightarrow> 'a list" where
+  "rev_aux acc [] = acc" |
+  "rev_aux acc (x # xs) = rev_aux (x # acc) xs"
+
+case_of_simps rev_aux_eq : rev_aux.simps
+function_compile_nat rev_aux_eq
+
+
+paragraph \<open>rev\<close>
+
+lemma rev_eq_rev_aux: "List.rev xs @ ys = local.rev_aux ys xs"
+  by (induction ys xs rule: rev_aux.induct) auto
+
+lemma rev_eq_rev_aux0: "List.rev xs = rev_aux [] xs"
+  using rev_eq_rev_aux[where ys = "[]"] by auto
+
+function_compile_nat rev_eq_rev_aux0
+
+
+paragraph \<open>append\<close>
+
+lemma append_eq_rev_aux: "List.append xs ys = rev_aux ys (rev xs)"
+  unfolding rev_eq_rev_aux[symmetric] by simp
+
+function_compile_nat append_eq_rev_aux
+
+
+paragraph \<open>zip\<close>
+
+fun zip_aux :: "('a \<times> 'b) list \<Rightarrow> 'a list \<Rightarrow> 'b list \<Rightarrow> ('a \<times> 'b) list" where
+  "zip_aux acc [] _ = acc" |
+  "zip_aux acc _ [] = acc" |
+  "zip_aux acc (x # xs) (y # ys) = zip_aux ((x, y) # acc) xs ys"
+
+lemma zip_eq_zip_aux: "rev zs @ List.zip xs ys = rev (zip_aux zs xs ys)"
+  apply (induction zs xs ys rule: zip_aux.induct)
+  unfolding rev_eq_rev_aux[symmetric] by auto
+
+lemma zip_eq_zip_aux0: "List.zip xs ys = rev (zip_aux [] xs ys)"
+  using zip_eq_zip_aux[where zs = "[]"]
+  unfolding rev_eq_rev_aux[symmetric] by auto
+
+case_of_simps zip_aux_eq : zip_aux.simps
+function_compile_nat zip_aux_eq
+function_compile_nat zip_eq_zip_aux0 (* TODO: this step is quite a bit slower *)
+
+
+subsection \<open>Association Lists\<close>
+
+fun assoc_lookup :: "'k \<Rightarrow> ('k \<times> 'v) list \<Rightarrow> 'v option" where
+  "assoc_lookup _ [] = None" |
+  "assoc_lookup x ((k, v) # xs) = (if x = k then Some v else assoc_lookup k xs)"
+
+case_of_simps assoc_lookup_eq : assoc_lookup.simps
+function_compile_nat assoc_lookup_eq
 
 end
 
 context HOL_To_IMP_Minus
 begin
 
-compile_nat Nil_nat_def
-HOL_To_IMP_Minus_correct Nil_nat by cook
+(* Currently we have a problem with the 'unconditional_nat', which is supposed to
+   remove the assumptions and TYPE arguments generated by 'function_compile_nat'.
+   If we use it to transform f into f', and want to use it to transform g, which calls f,
+   into g', then g' will must somehow reference f' instead of f.
+   Thus, we can't use the command on functions that use generated helper functions. *)
+
+section \<open>Bool\<close>
+
+compile_nat True_nat_def
+HOL_To_IMP_Minus_correct True_nat by cook
+
+compile_nat False_nat_def
+HOL_To_IMP_Minus_correct False_nat by cook
+
+
+section \<open>Pair\<close>
+
+compile_nat Pair_nat_def
+HOL_To_IMP_Minus_correct Pair_nat by cook
+
+lemmas fst_nat_eq_unfolded = HOL_To_HOL_Nat.fst_nat_eq_unfolded[simplified case_prod_nat_def]
+unconditional_nat fst_nat_eq_unfolded
+compile_nat fst_nat_unconditional.simps
+HOL_To_IMP_Minus_correct fst_nat_unconditional by cook
+
+lemmas snd_nat_eq_unfolded = HOL_To_HOL_Nat.snd_nat_eq_unfolded[simplified case_prod_nat_def]
+unconditional_nat snd_nat_eq_unfolded
+compile_nat snd_nat_unconditional.simps
+HOL_To_IMP_Minus_correct snd_nat_unconditional by cook
+
+
+section \<open>Three-way compare\<close>
+
+compile_nat LT_nat_def
+HOL_To_IMP_Minus_correct LT_nat by cook
+
+compile_nat EQ_nat_def
+HOL_To_IMP_Minus_correct EQ_nat by cook
+
+compile_nat GT_nat_def
+HOL_To_IMP_Minus_correct GT_nat by cook
+
+
+section\<open>Comparison (nat)\<close>
+
+lemmas leq_aux_nat_eq = HOL_To_HOL_Nat.leq_aux_nat_eq_unfolded[simplified case_nat_eq_if]
+unconditional_nat leq_aux_nat_eq
+declare leq_aux_nat_unconditional.simps [simp del]
+compile_nat leq_aux_nat_unconditional.simps
+HOL_To_IMP_Minus_correct leq_aux_nat_unconditional by (cook mode = tailcall)
+
+unconditional_nat HOL_To_HOL_Nat.leq_eq_leq_aux
+declare less_eq_unconditional.simps [simp del]
+(* TODO: ( <= ) needs helper function leq_aux *)
+(* compile_nat less_eq_unconditional.simps *)
+(* HOL_To_IMP_Minus_correct less_eq_unconditional by cook *)
+
+
+section \<open>Option\<close>
+
+compile_nat None_nat_def
+HOL_To_IMP_Minus_correct None_nat by cook
+
+compile_nat Some_nat_def
+HOL_To_IMP_Minus_correct Some_nat by cook
+
+
+paragraph \<open>is_some\<close>
+
+lemmas is_some_nat_eq = HOL_To_HOL_Nat.is_some_nat_eq_unfolded[simplified case_option_nat_def]
+unconditional_nat is_some_nat_eq
+declare is_some_nat_unconditional.simps [simp del]
+compile_nat is_some_nat_unconditional.simps
+HOL_To_IMP_Minus_correct is_some_nat_unconditional by cook
+
+paragraph \<open>get_some\<close>
+
+lemmas get_some_nat_eq = HOL_To_HOL_Nat.get_some_nat_eq_unfolded[simplified case_option_nat_def]
+unconditional_nat get_some_nat_eq
+declare get_some_nat_unconditional.simps [simp del]
+compile_nat get_some_nat_unconditional.simps
+HOL_To_IMP_Minus_correct get_some_nat_unconditional by cook
+
+
+section\<open>Lists\<close>
+
 compile_nat Cons_nat_def
 HOL_To_IMP_Minus_correct Cons_nat by cook
 
-(*problem: only got a conditional equation. We have to specify an unconditional one and prove it to
-be related to the original HOL function*)
+compile_nat Nil_nat_def
+HOL_To_IMP_Minus_correct Nil_nat by cook
+
+paragraph \<open>length\<close>
+
+lemmas length_aux_nat_eq = HOL_To_HOL_Nat.length_aux_nat_eq_unfolded[simplified case_list_nat_def]
+unconditional_nat length_aux_nat_eq
+declare length_aux_nat_unconditional.simps [simp del]
+compile_nat length_aux_nat_unconditional.simps
+HOL_To_IMP_Minus_correct length_aux_nat_unconditional by (cook mode = tailcall)
+
+(* TODO: this ends up getting named size_* *)
+lemmas length_nat_eq = HOL_To_HOL_Nat.size_nat_eq_unfolded[simplified case_list_nat_def]
+(* unconditional_nat length_nat_eq *)
+(* declare length_nat_unconditional.simps [simp del] *)
+(* compile_nat length_nat_unconditional.simps *)
+(* HOL_To_IMP_Minus_correct length_nat_unconditional by cook *)
+
+
+paragraph\<open>compare_lengths\<close>
+
+lemmas compare_lengths_nat_eq = HOL_To_HOL_Nat.compare_lengths_nat_eq_unfolded[simplified case_list_nat_def]
+unconditional_nat compare_lengths_nat_eq
+declare compare_lengths_nat_unconditional.simps [simp del]
+compile_nat compare_lengths_nat_unconditional.simps
+HOL_To_IMP_Minus_correct compare_lengths_nat_unconditional by (cook mode = tailcall)
+
+
+paragraph \<open>rev_aux\<close>
+
+(* FIXME: we could use the equation without unfolding case_list_nat_def if we prove
+   congruence lemmas for case_list_nat (otherwise the function package cannot prove termination) *)
+lemmas rev_aux_nat_eq = HOL_To_HOL_Nat.rev_aux_nat_eq_unfolded[simplified case_list_nat_def]
+unconditional_nat rev_aux_nat_eq
+declare rev_aux_nat_unconditional.simps [simp del]
+compile_nat rev_aux_nat_unconditional.simps
+HOL_To_IMP_Minus_correct rev_aux_nat_unconditional by (cook mode = tailcall)
+
+(* Problem: We have obtained an unconditional equation. However, we
+   still have to prove it to be related to the original HOL function.
+   TODO: how to prove the two functions to be related? Currently, we are
+   missing the right lemmas to make it automatic. *)
+
 context
   fixes xs ys and xs' ys' :: "('a :: compile_nat) list"
   assumes rels: "Rel_nat xs xs'" "Rel_nat ys ys'"
 begin
-term HOL_To_HOL_Nat.rev_tail_aux_nat
-print_statement HOL_To_HOL_Nat.rev_tail_aux_nat_eq_unfolded
-print_statement HOL_To_HOL_Nat.rev_tail_aux_nat_eq_unfolded[OF rels, unfolded case_list_nat_def]
+  term HOL_To_HOL_Nat.rev_aux_nat
+  print_statement HOL_To_HOL_Nat.rev_aux_nat_eq_unfolded
+  print_statement HOL_To_HOL_Nat.rev_aux_nat_eq_unfolded[OF rels, unfolded case_list_nat_def]
 end
 
-(*FIXME: we could use the equation without unfolding case_list_nat_def if we prove congruence lemmas
-for case_list_nat (otherwise the function package cannot prove termination)*)
-fun rev_tail_aux_nat' :: "nat \<Rightarrow> nat \<Rightarrow> nat" where
-  "rev_tail_aux_nat' xs acc = (if fst_nat xs = 0 then acc else
-    rev_tail_aux_nat' (snd_nat (snd_nat xs)) (Cons_nat (fst_nat (snd_nat xs)) acc))"
-declare rev_tail_aux_nat'.simps[simp del]
+lemma natify_list_simps_Nil: "natify [] = Nil_nat"
+  by (subst natify_list.simps) simp
 
-compile_nat rev_tail_aux_nat'.simps
-HOL_To_IMP_Minus_correct rev_tail_aux_nat' by (cook mode = tailcall)
+lemma natify_list_simps_Cons: "natify (x # xs) = Cons_nat (natify x) (natify xs)"
+  by (subst natify_list.simps) simp
 
-(*TODO: how to prove the two functions to be related? Currently, we are missing the right lemmas to
-make it automatic*)
+(* we would need these elimination/destruction lemmas to automate the proofs *)
+
 lemma Rel_nat_NilE:
-  assumes "Rel_nat xs []"
+  assumes rel: "Rel_nat xs []"
   obtains "xs = Nil_nat"
-  using assms
-  apply (subst (asm) Rel_nat_iff_eq_natify)
-  apply (subst (asm) natify_list.simps)
-  apply (simp (no_asm_use))
-  by assumption
+  (* this proof is not "optimal", but can hopefully be mechanically derived for each constructor *)
+  apply standard
+  apply (subst rel[simplified Rel_nat_iff_eq_natify])
+    apply (subst natify_list_simps_Nil)
+    apply (rule refl)
+   apply ((rule Rel_nat_natify_self)+)?
+  done
 
 lemma Rel_nat_ConsE:
-  assumes "Rel_nat xs (y # ys)"
+  assumes rel: "Rel_nat xs (y # ys)"
   obtains z zs where "xs = Cons_nat z zs" "Rel_nat z y" "Rel_nat zs ys"
-  using assms
-  (* apply (subst (asm) (3) Rel_nat_iff_eq_natify)
-  apply (subst (asm) natify_list.simps)
-  apply (simp (no_asm_use))
-  by assumption *)
-  sorry
+  apply standard
+  apply (subst rel[simplified Rel_nat_iff_eq_natify])
+    apply (subst natify_list_simps_Cons)
+    apply (rule refl)
+   apply ((rule Rel_nat_natify_self)+)?
+  done
 
 lemma Rel_nat_NilD:
   assumes "Rel_nat xs []"
@@ -86,25 +335,25 @@ lemma Rel_nat_ConsD:
   shows "\<exists>z zs. xs = Cons_nat z zs \<and> Rel_nat z y \<and> Rel_nat zs ys"
   using assms Rel_nat_ConsE by blast
 
-(*probably best approach: use induction on the original function's definition*)
+(* probably best approach: use induction on the original function's definition *)
 lemma
   fixes xs acc and xs' acc' :: "('a :: compile_nat) list"
   assumes rels: "Rel_nat xs xs'" "Rel_nat acc acc'"
-  shows "Rel_nat (rev_tail_aux_nat' xs acc) (HOL_To_HOL_Nat.rev_tail_aux xs' acc')"
+  shows "Rel_nat (rev_aux_nat_unconditional xs acc) (HOL_To_HOL_Nat.rev_aux xs' acc')"
   using assms
-  apply (induction xs' acc' arbitrary: xs acc rule: HOL_To_HOL_Nat.rev_tail_aux.induct)
+  apply (induction xs' acc' arbitrary: xs acc rule: HOL_To_HOL_Nat.rev_aux.induct)
 
-  apply (subst HOL_To_HOL_Nat.rev_tail_aux.simps)
+  apply (subst HOL_To_HOL_Nat.rev_aux.simps)
   apply (frule Rel_nat_NilD Rel_nat_ConsD; (elim exE)?)
   apply hypsubst
-  apply (subst rev_tail_aux_nat'.simps)
+  apply (subst rev_aux_nat_unconditional.simps)
   apply (simp (no_asm) add: Nil_nat_def Cons_nat_def,
    (simp (no_asm) only: flip: Nil_nat_def Cons_nat_def)?)
 
-  apply (subst HOL_To_HOL_Nat.rev_tail_aux.simps)
+  apply (subst HOL_To_HOL_Nat.rev_aux.simps)
   apply (frule Rel_nat_NilD Rel_nat_ConsD; (elim conjE exE)?)
   apply hypsubst
-  apply (subst rev_tail_aux_nat'.simps)
+  apply (subst rev_aux_nat_unconditional.simps)
   apply (simp (no_asm) add: Nil_nat_def Cons_nat_def,
    (simp (no_asm) only: flip: Nil_nat_def Cons_nat_def)?)
   subgoal premises p
@@ -114,6 +363,37 @@ lemma
     apply (metis Rel_nat_Cons_nat rel_funD)
     done
   done
+
+
+paragraph \<open>rev\<close>
+
+(* TODO: aux function rev_aux needed for rev *)
+
+
+paragraph \<open>append\<close>
+
+(* TODO: aux function rev_aux needed for append *)
+
+
+paragraph \<open>zip\<close>
+
+lemmas zip_aux_nat_eq = HOL_To_HOL_Nat.zip_aux_nat_eq_unfolded[simplified case_list_nat_def]
+unconditional_nat zip_aux_nat_eq
+declare zip_aux_nat_unconditional.simps [simp del]
+compile_nat zip_aux_nat_unconditional.simps
+HOL_To_IMP_Minus_correct zip_aux_nat_unconditional by (cook mode = tailcall)
+
+
+(* TODO: aux function rev needed for zip *)
+
+
+subsection \<open>Association Lists\<close>
+
+lemmas assoc_lookup_nat_eq = HOL_To_HOL_Nat.assoc_lookup_nat_eq_unfolded[simplified case_list_nat_def case_prod_nat_def]
+unconditional_nat assoc_lookup_nat_eq
+declare assoc_lookup_nat_unconditional.simps [simp del]
+compile_nat assoc_lookup_nat_unconditional.simps
+HOL_To_IMP_Minus_correct assoc_lookup_nat_unconditional by (cook mode = tailcall)
 
 end
 
